fix: wrong free_ pre-conditions

TheoryTask/qcp-binary-democases/QCP_examples/sll_lib.c
@@ -30,7 +30,7 @@ struct sll * cons_list(unsigned int data, struct sll * next)
 }
 
 void free_list_node(struct sll * p)
-/*@ Require emp
+/*@ Require exists d n, p -> data == d && p -> next == n && emp
     Ensure emp
 */;
 
@@ -157,15 +157,17 @@ struct sllb * app_list_box(struct sllb * b1, struct sllb * b2)
     /*@ sllb(b1, l1) * sllb(b2, l2)
         which implies
         exists h1 pt1 h2 pt2,
-            b1 -> head == h1 && b1 -> ptail == pt1 && 
+            b1 -> head == h1 && b1 -> ptail == pt1 &&
             b2 -> head == h2 && b2 -> ptail == pt2 &&
             sllbseg(&(b1 -> head), pt1, l1) * store(pt1, struct sll *, 0) *
             sllbseg(&(b2 -> head), pt2, l2) * store(pt2, struct sll *, 0)
     */
-    * (b1 -> ptail) = b2 -> head;
-    if (b2 -> head != (struct sll *) 0)
+    struct sll * h2 = b2 -> head;
+    struct sll ** pt2 = b2 -> ptail;
+    * (b1 -> ptail) = h2;
+    if (h2 != (struct sll *) 0)
     {
-        b1 -> ptail = b2 -> ptail;
+        b1 -> ptail = pt2;
     }
     free_sllb(b2);
     return b1;
